term definition

Unification.thy
@@ -1,6 +1,23 @@
 chapter {* camr project *}
 
 theory Unification imports Main begin
-(*comment*)
+
+(* Assignment 1 *)
+
+datatype ('f, 'v) "term" = Var 'v | Fun 'f "('f, 'v) term list"
+
+fun fv :: "('f, 'v) term \<Rightarrow> 'v set" where
+
+type_synonym ('f, 'v) subst = "'v \<Rightarrow> ('f, 'v) term"
+
+fun sapply :: "('f, 'v) subst \<Rightarrow> ('f, 'v) term \<Rightarrow> ('f, 'v) term" (infixr "\<cdot>" 67) where 
+
+fun scomp :: "('f, 'v) subst \<Rightarrow> ('f, 'v) subst \<Rightarrow> ('f, 'v) subst" (infixl "\<circ>s" 75) where
+
+lemma fv_sapply: "fv (\<sigma> \<cdot> t) = (\<Union>x \<in> fv t. fv (\<sigma> x))"
+
+
+
+
 
 end
